HepLean/PerturbationTheory/Contractions/ExtractEquiv.lean
@@ -1,0 +1,110 @@
+/-
+Copyright (c) 2025 Joseph Tooby-Smith. All rights reserved.
+Released under Apache 2.0 license as described in the file LICENSE.
+Authors: Joseph Tooby-Smith
+-/
+import HepLean.PerturbationTheory.Contractions.Insert
+/-!
+
+# Equivalence extracting element from contraction
+
+
+-/
+
+namespace FieldStruct
+variable {𝓕 : FieldStruct}
+
+namespace ContractionsNat
+variable {n : ℕ} (c : ContractionsNat n)
+open HepLean.List
+open HepLean.Fin
+
+
+lemma extractEquiv_equiv {c1 c2 : (c : ContractionsNat n) × Option c.uncontracted}
+    (h : c1.1 = c2.1) (ho : c1.2 = uncontractedCongr (by rw [h]) c2.2) : c1 = c2 := by
+  cases c1
+  cases c2
+  simp_all
+  simp at h
+  subst h
+  simp [uncontractedCongr]
+  rename_i a
+  match a with
+  | none => simp
+  | some a =>
+    simp
+    ext
+    simp
+
+
+def extractEquiv (i : Fin n.succ) : ContractionsNat n.succ ≃
+    (c : ContractionsNat n) × Option c.uncontracted  where
+  toFun := fun c => ⟨erase c i, getDualErase c i⟩
+  invFun := fun ⟨c, j⟩ => insert c i j
+  left_inv f := by
+    simp
+  right_inv f := by
+    refine extractEquiv_equiv ?_ ?_
+    simp
+    simp
+    have h1 := insert_getDualErase f.fst i f.snd
+    exact insert_getDualErase _ i _
+
+lemma extractEquiv_symm_none_uncontracted (i : Fin n.succ)  (c : ContractionsNat n) :
+    ((extractEquiv i).symm ⟨c, none⟩).uncontracted =
+    (Insert.insert i (c.uncontracted.map i.succAboveEmb)) := by
+  exact insert_none_uncontracted c i
+
+@[simp]
+lemma extractEquiv_apply_congr_symm_apply {n m : ℕ} (k : ℕ)
+    (hnk :  k < n.succ) (hkm : k < m.succ) (hnm : n = m) (c : ContractionsNat n)
+     (i  : c.uncontracted) :
+    congr (by rw [hnm]) ((extractEquiv ⟨k, hkm⟩
+    (congr (by rw [hnm]) ((extractEquiv ⟨k, hnk⟩).symm ⟨c, i⟩)))).1 = c := by
+  subst hnm
+  simp
+
+instance fintype_zero : Fintype (ContractionsNat 0) where
+  elems := {nil}
+  complete := by
+    intro c
+    simp
+    apply Subtype.eq
+    simp [nil]
+    ext a
+    apply Iff.intro
+    · intro h
+      have hc := c.2.1 a h
+      rw [Finset.card_eq_two] at hc
+      obtain ⟨x, y, hxy, ha⟩ := hc
+      exact Fin.elim0 x
+    · simp
+
+lemma sum_contractionsNat_nil (f : ContractionsNat 0 → M) [AddCommMonoid M] :
+    ∑ c, f c = f nil := by
+  rw [Finset.sum_eq_single_of_mem]
+  simp
+  intro b hb
+  fin_cases b
+  simp
+
+instance fintype_succ : (n : ℕ) → Fintype (ContractionsNat n)
+  | 0 => fintype_zero
+  | Nat.succ n => by
+    letI := fintype_succ n
+    exact Fintype.ofEquiv _ (extractEquiv 0).symm
+
+
+lemma sum_extractEquiv_congr [AddCommMonoid M] {n m : ℕ} (i : Fin n) (f : ContractionsNat n → M)
+    (h : n = m.succ) :
+    ∑ c, f c = ∑ (c : ContractionsNat m), ∑ (k : Option c.uncontracted),
+    f (congr h.symm ((extractEquiv (finCongr h i)).symm ⟨c, k⟩))  := by
+  subst h
+  simp only [finCongr_refl, Equiv.refl_apply, congr_refl]
+  rw [← (extractEquiv i).symm.sum_comp]
+  rw [Finset.sum_sigma']
+  rfl
+
+end ContractionsNat
+
+end FieldStruct
