HepLean/PerturbationTheory/Contractions/TimeContract.lean
@@ -4,6 +4,7 @@ Released under Apache 2.0 license as described in the file LICENSE.
 Authors: Joseph Tooby-Smith
 -/
 import HepLean.PerturbationTheory.Contractions.Sign
+import HepLean.PerturbationTheory.FieldStruct.TimeContraction
 /-!
 
 # Time contractions
